pancake/semantics/panHoareScript.sml
@@ -1,0 +1,383 @@
+(*
+  A program logic for pancake in the Hoare/Floyd style.
+*)
+
+open preamble panLangTheory panPropsTheory;
+local open alignmentTheory
+           miscTheory
+           wordLangTheory
+           ffiTheory in end;
+
+val _ = new_theory "panHoare";
+val _ = set_grammar_ancestry [
+  "panLang", "panSem", "ffi" ]
+
+
+
+Datatype:
+  hoare_context = <|
+      exceptions_ok     :    eid -> bool
+    ; ffi_rely          :    io_event list ->
+                             (ffiname # word8 list # word8 list) ->
+                             ('ffi oracle_result) -> bool
+    ; ffi_guarantee     :    io_event list ->
+                             (ffiname # word8 list # word8 list) -> bool
+    ; termination       :    bool
+    ; triples           :    mlstring |-> ((('a, 'ffi) state -> bool) # (('a, 'ffi) state -> bool))
+  |>
+End
+
+(* should this be presented syntactically via Inductive? *)
+Definition eval_logic_def:
+  eval_logic G P exp v Q = (!s. P s ==> ?x. eval s exp = SOME x /\
+    Q (s with locals := (s.locals |+ (v, x))))
+End
+
+Theorem eval_logic_elim = hd (RES_CANON eval_logic_def)
+
+Definition opt_op_precond_def:
+  opt_op_precond P f Q = (!s. P s ==> ?x. f s = SOME x /\ Q x s)
+End
+
+Theorem opt_op_precond_elim = hd (RES_CANON opt_op_precond_def)
+
+Inductive hoare_logic:
+
+[hoare_logic_weaken_pre:]
+  (! Q.
+    (!s. P s ==> Q s) /\
+    hoare_logic G Q p R ==>
+    hoare_logic G P p R
+  )
+
+[hoare_logic_equiv:]
+  (! Q.
+    (!s r s1. P s /\ evaluate (p, s) = (r, s1) ==>
+        ?s2. evaluate (p2, s) = (r, s2) /\ empty_locals s2 = empty_locals s1 /\
+            (((r = NONE) \/ (r = SOME Break) \/ (r = SOME Continue)) ==> s1 = s2)) /\
+    hoare_logic G Q p2 R ==>
+    hoare_logic G (\s. P s /\ Q s) p R
+  )
+
+[hoare_logic_Skip:]
+  (
+    hoare_logic G P Skip P
+  )
+
+[hoare_logic_Dec:]
+  (
+    ! Q.
+    eval_logic G P e v Q /\
+    (!prev. hoare_logic G Q p
+        (\s. R (s with locals := res_var s.locals (v, prev))))
+    ==>
+    hoare_logic G P (Dec v e p) R
+  )
+
+[hoare_logic_Assign:]
+  (
+    eval_logic G P e v Q ==>
+    hoare_logic G (\s. P s /\
+            OPTION_MAP shape_of (FLOOKUP s.locals v) =
+            SOME (exp_shape (FMAP_MAP2 (shape_of o SND) s.locals) e))
+        (Assign v e) Q
+  )
+
+[hoare_logic_Seq:]
+  (
+    ! Q.
+    hoare_logic G P p1 Q /\
+    hoare_logic G Q p2 R ==>
+    hoare_logic G P (Seq p1 p2) R
+  )
+
+[hoare_logic_While:]
+  (
+    ! Q.
+    eval_logic_word G P e (\x s. if x = 0w then R s else Q (dec_clock s)) /\
+    hoare_logic G Q p P ==>
+    hoare_logic G P (While e p) R
+  )
+
+(* [hoare_logic_TailCall:]
+  (
+    ! Q1 Q2 Q3.
+    eval_logic G P target ...
+    eval_logic G ... (Struct args) ...
+    opt_op_precond ... (\s. case target_v of ValLabel f =>
+        lookup_code s.code fname args_v
+      | _ => NONE) ...
+    hoare_logic
+
+    hoare_logic G Q p P ==>
+    hoare_logic G P (Call NONE target args) R
+  )
+
+[hoare_logic_ExtCall:]
+  ( ! Q1 Q2 Q3 Q4.
+    eval_logic_word G P ptr1 Q1 /\
+    (!x1. eval_logic_word G (Q1 x1) len1 (Q2 x1)) /\
+    (!x1 x2. eval_logic_word G (Q2 x1 x2) ptr2 (Q3 x1 x2)) /\
+    (!x1 x2 x3. eval_logic_word G (Q3 x1 x2 x3) len2 (Q4 x1 x2 x3)) /\
+    (! p1 sz1 p2 sz2. opt_op_precond (Q4 p1 sz1 p2 sz2)
+        (\s. read_bytearray p1 (w2n sz1) (mem_load_byte s.memory s.memaddrs s.be))
+        (Q5 p1 sz1 p2 sz2)) /\
+    (! p1 sz1 p2 sz2 b1. opt_op_precond (Q5 p1 sz1 p2 sz2 b1)
+        (\s. read_bytearray p2 (w2n sz2) (mem_load_byte s.memory s.memaddrs s.be))
+        (\b2 s. let ffi_nm = ExtCall (explode f) in
+            if explode f = "" then R s else
+            G.ffi_guarantee s.ffi.io_events (ffi_nm, b1, b2) /\
+            (! rv. G.ffi_rely s.ffi.io_events (ffi_nm, b1, b2) rv ==>
+                (case rv of Oracle_final _ => F
+                    | Oracle_return ffi l => LENGTH l = LENGTH b2 /\
+                    let ev = IO_event ffi_nm b1 (ZIP (b2, l)) in
+                    R (s with <| memory := write_bytearray p2 l s.memory s.memaddrs s.be;
+                        ffi := s.ffi with <| ffi_state := ffi; io_events := s.ffi.io_events ++ [ev] |> |>)
+    )))) ==>
+    hoare_logic G P (ExtCall f ptr1 len1 ptr2 len2) R
+  )
+*)
+
+End
+
+val eval_ind_rule =
+  evaluate_ind |> Q.SPEC `UNCURRY P` |> REWRITE_RULE [UNCURRY_DEF] |> Q.GEN `P`
+
+Theorem evaluate_While_inv_final:
+  (! s. P s ==> (?w. eval s e = SOME (ValWord w)) /\
+    (! w r s'. eval s e = SOME (ValWord w) ==> w <> 0w ==>
+        evaluate (p, dec_clock s) = (r, s') ==>
+        (r = SOME TimeOut /\ Q s' \/ (r = NONE /\ P s' /\ Q (empty_locals s'))))) ==>
+  ! s res s'.
+  evaluate (While e p, s) = (res, s') ==>
+  P s /\ Q (empty_locals s) ==>
+  (res = SOME TimeOut /\ Q s') \/
+  (res = NONE /\ P s' /\ eval s' e = SOME (ValWord 0w))
+Proof
+  disch_tac \\ gen_tac
+  \\ measureInduct_on `s.clock`
+  \\ rpt GEN_TAC
+  \\ ONCE_REWRITE_TAC [evaluate_def]
+  \\ rpt disch_tac
+  \\ fs []
+  \\ last_x_assum drule
+  \\ rpt disch_tac
+  \\ gs []
+  \\ fs [CaseEq "bool"]
+  \\ rpt (pairarg_tac \\ fs [])
+  \\ gs []
+  \\ last_x_assum (drule_at (Pat `evaluate (While _ _, _) = _`))
+  \\ fs [dec_clock_def]
+  \\ imp_res_tac evaluate_clock
+  \\ fs []
+QED
+
+Definition events_meet_guarantee_def:
+  events_meet_guarantee g evs =
+  (!i. i < LENGTH evs ==>
+    case (EL i evs) of IO_event ffi_nm const_bs upd_bs =>
+    g (TAKE i evs) (ffi_nm, const_bs, MAP FST upd_bs)
+  )
+End
+
+Theorem events_meet_guarantee_snoc:
+  events_meet_guarantee g (evs ++ [ev]) =
+  (events_meet_guarantee g evs /\
+    (case ev of IO_event ffi_nm const_bs upd_bs =>
+        g evs (ffi_nm, const_bs, MAP FST upd_bs)))
+Proof
+  simp [events_meet_guarantee_def, GSYM ADD1, prim_recTheory.LESS_THM]
+  \\ simp [DISJ_IMP_THM, FORALL_AND_THM, EL_APPEND]
+  \\ simp [CONJ_COMM, TAKE_APPEND]
+  \\ simp (RES_CANON arithmeticTheory.SUB_EQ_0)
+QED
+
+Definition ffi_rely_guarantee_def:
+  ffi_rely_guarantee r g ffi =
+  (! evs2 ffi_nm const_bs upd_bs.
+    g (ffi.io_events ++ evs2) (ffi_nm, const_bs, upd_bs) ==>
+    let st = FOLDL (\st ev. case ev of
+        IO_event ffi_nm const_bs upd_bs => (case ffi.oracle ffi_nm st const_bs (MAP FST upd_bs) of
+            Oracle_return st' _ => st')) ffi.ffi_state evs2 in
+    r (ffi.io_events ++ evs2) (ffi_nm, const_bs, upd_bs)
+        (ffi.oracle ffi_nm st const_bs upd_bs))
+End
+
+Theorem ffi_rely_guarantee_step:
+  ffi_rely_guarantee r g ffi ==>
+    g ffi.io_events (ffi_nm, const_bs, upd_bs) ==>
+    r ffi.io_events (ffi_nm, const_bs, upd_bs)
+        (ffi.oracle ffi_nm ffi.ffi_state const_bs upd_bs) /\
+    (!st bs2. ffi.oracle ffi_nm ffi.ffi_state const_bs upd_bs =
+            Oracle_return st bs2 /\ LENGTH bs2 = LENGTH upd_bs ==>
+        ffi_rely_guarantee r g (ffi with <| ffi_state := st;
+                io_events := ffi.io_events ++ [IO_event ffi_nm const_bs (ZIP (upd_bs, bs2))] |>))
+Proof
+  rw [ffi_rely_guarantee_def]
+  >- (
+    first_x_assum (qspec_then `[]` mp_tac)
+    \\ simp []
+  )
+  >- (
+    full_simp_tac bool_ss [GSYM APPEND_ASSOC]
+    \\ last_x_assum drule
+    \\ simp [MAP_ZIP]
+  )
+QED
+
+Theorem mem_store_byte_same:
+  mem_load_byte m dm be ptr = SOME b ==>
+  mem_store_byte m dm be ptr b = SOME m
+Proof
+  rw [mem_load_byte_def]
+  \\ gvs [CaseEq "word_lab", get_byte_def]
+  \\ simp [mem_store_byte_def, set_byte_def]
+  \\ cheat
+QED
+
+Theorem write_bytearray_same:
+  ! sz ptr m x y bs.
+  read_bytearray ptr sz (mem_load_byte m x y) = SOME bs ==>
+  write_bytearray ptr bs m x y = m
+Proof
+  Induct \\ simp [read_bytearray_def, write_bytearray_def]
+  \\ rw []
+  \\ fs [CaseEq "option"]
+  \\ gvs [write_bytearray_def]
+  \\ simp [mem_store_byte_same]
+QED
+
+Overload ffi_g_ok[local] = ``\G ffi.
+    ffi_rely_guarantee G.ffi_rely G.ffi_guarantee ffi``;
+
+Overload ffi_g_imp[local] = ``\G s s'.
+    events_meet_guarantee G.ffi_guarantee s.ffi.io_events ==>
+    events_meet_guarantee G.ffi_guarantee s'.ffi.io_events
+    ``;
+
+Triviality empty_locals_eq_IMP:
+  empty_locals s = empty_locals s2 ==>
+  ?l. s = (s2 with locals := l)
+Proof
+  simp [state_component_equality, empty_locals_def]
+QED
+
+Theorem hoare_logic_sound:
+
+  ! P p Q.
+  hoare_logic G P p Q ==>
+  (! s res s'. evaluate (p, s) = (res, s') ==> P s ==>
+    ffi_g_ok G s.ffi ==>
+    (res = SOME TimeOut \/ (res = NONE /\
+        Q s' /\ ffi_g_ok G s'.ffi)) /\
+    (ffi_g_imp G s s')
+  )
+
+Proof
+
+  ho_match_mp_tac (Q.SPEC `G` hoare_logic_ind)
+  \\ rpt conj_tac
+  \\ rpt (gen_tac ORELSE disch_tac)
+  >- (
+    metis_tac []
+  )
+
+  >- (
+    fs []
+    \\ res_tac \\ res_tac \\ fs []
+    \\ imp_res_tac empty_locals_eq_IMP
+    \\ gvs []
+  )
+
+  >- (
+    gs [evaluate_def]
+  )
+  >- (
+    fs [evaluate_def]
+    \\ drule_then (drule_then assume_tac) eval_logic_elim
+    \\ gs []
+    \\ (pairarg_tac \\ fs [])
+    \\ first_x_assum (drule_then drule)
+    \\ rw []
+  )
+  >- (
+    fs [evaluate_def]
+    \\ drule_then (drule_then assume_tac) eval_logic_elim
+    \\ gvs []
+    \\ imp_res_tac eval_exp_shape
+    \\ fs [is_valid_value_def]
+    \\ gvs []
+  )
+  >- (
+    fs [evaluate_def]
+    \\ pairarg_tac \\ fs []
+    \\ first_x_assum (drule_then (drule_then assume_tac))
+    \\ gvs []
+    \\ first_x_assum (drule_then (drule_then assume_tac))
+    \\ metis_tac []
+  )
+  >- (
+    dxrule_at (Pat `evaluate (While _ _, _) = _`) evaluate_While_inv_final
+    \\ disch_then (qspec_then `ffi_g_imp G s` mp_tac)
+    \\ disch_then (qspec_then `\s'. P s' /\ ffi_g_ok G s'.ffi /\ ffi_g_imp G s s'` mp_tac)
+    \\ impl_tac \\ fs []
+    >- (
+      simp [empty_locals_def]
+      \\ rpt (gen_tac ORELSE disch_tac)
+      \\ fs []
+      \\ drule_then (drule_then assume_tac) eval_logic_word_elim
+      \\ fs []
+      \\ rw []
+      \\ first_x_assum drule
+      \\ gs [dec_clock_def]
+    )
+    \\ strip_tac
+    \\ fs []
+    \\ drule_then (drule_then assume_tac) eval_logic_word_elim
+    \\ gs []
+  )
+
+  >- (
+    (* ExtCall *)
+    fs [eval_logic_word_def, eval_logic_def]
+    \\ rpt (last_x_assum (drule_then strip_assume_tac)
+        \\ fs [eval_logic_word_elim_helper])
+    \\ gvs []
+    \\ last_x_assum mp_tac
+    \\ simp [opt_op_precond_def]
+    \\ disch_then (drule_then strip_assume_tac)
+    \\ last_x_assum mp_tac
+    \\ simp [opt_op_precond_def]
+    \\ disch_then (drule_then strip_assume_tac)
+    \\ fs [evaluate_def, ffiTheory.call_FFI_def]
+    \\ Cases_on `explode f = ""` \\ fs []
+    >- (
+      drule write_bytearray_same \\ simp []
+      \\ rw [] \\ fs []
+      \\ qmatch_goalsub_abbrev_tac `Q s2`
+      \\ qsuff_tac `s2 = s` \\ fs []
+      \\ fs [Abbr `s2`]
+      \\ simp [panSemTheory.state_component_equality]
+    )
+    \\ dxrule_then drule ffi_rely_guarantee_step
+    \\ strip_tac
+    \\ first_x_assum drule
+    \\ fs [CaseEq "ffi_result", CaseEq "oracle_result", CaseEq "bool"] \\ gvs []
+    \\ rw []
+    \\ simp [events_meet_guarantee_snoc, MAP_ZIP]
+  )
+
+QED
+
+Theorem hoare_logic_rules = LIST_CONJ (tl (BODY_CONJUNCTS hoare_logic_rules))
+
+
+Theorem eval_logic_Const:
+  eval_logic G (Q (ValWord c)) (Const c) Q
+Proof
+  simp [eval_logic_def, eval_def]
+QED
+
+
+
+
